src/axiomatic/TsoPFtoA4OBR.v
@@ -141,7 +141,42 @@ Proof.
           unfold v_gen. ss. rewrite <- H7. auto.
         }
         subst.
-        repeat rewrite <- join_r. ss.
+        repeat rewrite <- join_r. unfold FwdItem.read_view. condtac; ss. clear X0. inv e.
+        generalize (L.(LC).(FWDBANK) (ValA.val vloc)). s. i. des.
+        + rewrite <- TS in H2.
+          destruct eid as [tid2 eid2], eid1 as [tid1 eid1].
+          assert (tid1 = tid2).
+          { inv H. exploit RF2; eauto. i. des.
+            inv WRITE0. rename EID0 into WRITE0.
+            unfold Execution.label in WRITE0. ss.
+            rewrite PRE.(Valid.LABELS) in WRITE0.
+            rewrite IdMap.map_spec in WRITE0.
+            destruct (IdMap.find tid1 (Valid.aeus PRE)) eqn:FIND1; ss.
+            generalize (ATR tid1). intro ATR1. inv ATR1; try congr. des. simplify.
+            generalize (SIM tid1). intro SIM1. inv SIM1; simplify.
+            exploit sim_trace_last; try exact REL0. i. des. simplify.
+            exploit sim_trace_sim_th; try exact REL0; eauto. intro L1.
+            inv WRITE. inv WRITE1.
+            unfold Execution.label in EID0. ss.
+            rewrite PRE.(Valid.LABELS) in EID0.
+            rewrite IdMap.map_spec in EID0.
+            destruct (IdMap.find tid2 (Valid.aeus PRE)) eqn:FIND2; ss.
+            generalize (ATR tid2). intro ATR2. inv ATR2; try congr. des. simplify.
+            generalize (SIM tid2). intro SIM2. inv SIM2; simplify.
+            exploit sim_trace_last; try exact REL1. i. des. simplify.
+            exploit sim_trace_sim_th; try exact REL1; eauto. intro L2.
+            move H2 at bottom.
+            unfold v_gen in H2. ss.
+            rewrite <- H10, <- H16 in H2.
+            exploit L1.(WPROP2); eauto. i. des.
+            exploit L2.(WPROP2'); eauto. i. des.
+            exploit L1.(WPROP3); eauto. i. des.
+            exploit L2.(WPROP3); eauto. i. des.
+            rewrite x8, x15 in H2. inv H2.
+            rewrite H in x19. rewrite x12 in x19. inv x19. ss. }
+          subst.
+          inv WRITE. inv PO. ss. subst. inv H. inv H3. ss.
+        + rewrite H1. refl.
       - (* dob *)
         rename H1 into H.
         unfold Execution.dob in H. rewrite ? seq_assoc in *. des_union.
@@ -187,7 +222,42 @@ Proof.
           unfold v_gen. ss. rewrite <- H7. auto.
         }
         subst.
-        repeat rewrite <- join_r. ss.
+        repeat rewrite <- join_r. ss. unfold FwdItem.read_view. condtac; ss. clear X0. inv e.
+        generalize (L.(LC).(FWDBANK) (ValA.val vloc)). s. i. des.
+        + rewrite <- TS in H2.
+          destruct eid as [tid2 eid2], eid1 as [tid1 eid1].
+          assert (tid1 = tid2).
+          { inv H. exploit RF2; eauto. i. des.
+            inv WRITE0. rename EID0 into WRITE0.
+            unfold Execution.label in WRITE0. ss.
+            rewrite PRE.(Valid.LABELS) in WRITE0.
+            rewrite IdMap.map_spec in WRITE0.
+            destruct (IdMap.find tid1 (Valid.aeus PRE)) eqn:FIND1; ss.
+            generalize (ATR tid1). intro ATR1. inv ATR1; try congr. des. simplify.
+            generalize (SIM tid1). intro SIM1. inv SIM1; simplify.
+            exploit sim_trace_last; try exact REL0. i. des. simplify.
+            exploit sim_trace_sim_th; try exact REL0; eauto. intro L1.
+            inv WRITE. inv WRITE1.
+            unfold Execution.label in EID0. ss.
+            rewrite PRE.(Valid.LABELS) in EID0.
+            rewrite IdMap.map_spec in EID0.
+            destruct (IdMap.find tid2 (Valid.aeus PRE)) eqn:FIND2; ss.
+            generalize (ATR tid2). intro ATR2. inv ATR2; try congr. des. simplify.
+            generalize (SIM tid2). intro SIM2. inv SIM2; simplify.
+            exploit sim_trace_last; try exact REL1. i. des. simplify.
+            exploit sim_trace_sim_th; try exact REL1; eauto. intro L2.
+            move H2 at bottom.
+            unfold v_gen in H2. ss.
+            rewrite <- H10, <- H16 in H2.
+            exploit L1.(WPROP2); eauto. i. des.
+            exploit L2.(WPROP2'); eauto. i. des.
+            exploit L1.(WPROP3); eauto. i. des.
+            exploit L2.(WPROP3); eauto. i. des.
+            rewrite x8, x15 in H2. inv H2.
+            rewrite H in x19. rewrite x12 in x19. inv x19. ss. }
+          subst.
+          inv WRITE. inv PO. ss. subst. inv H. inv H3. ss.
+        + rewrite H1. refl.
       - (* dob *)
         rename H1 into H.
         unfold Execution.dob in H. rewrite ? seq_assoc in *. des_union.
@@ -254,7 +324,42 @@ Proof.
           unfold v_gen. ss. rewrite <- H7. auto.
         }
         subst.
-        repeat rewrite <- join_r. ss.
+        repeat rewrite <- join_r. ss. unfold FwdItem.read_view. condtac; ss. clear X0. inv e.
+        generalize (L.(LC).(FWDBANK) (ValA.val vloc)). s. i. des.
+        + rewrite <- TS in H2.
+          destruct eid as [tid2 eid2], eid1 as [tid1 eid1].
+          assert (tid1 = tid2).
+          { inv H. exploit RF2; eauto. i. des.
+            inv WRITE0. rename EID0 into WRITE0.
+            unfold Execution.label in WRITE0. ss.
+            rewrite PRE.(Valid.LABELS) in WRITE0.
+            rewrite IdMap.map_spec in WRITE0.
+            destruct (IdMap.find tid1 (Valid.aeus PRE)) eqn:FIND1; ss.
+            generalize (ATR tid1). intro ATR1. inv ATR1; try congr. des. simplify.
+            generalize (SIM tid1). intro SIM1. inv SIM1; simplify.
+            exploit sim_trace_last; try exact REL0. i. des. simplify.
+            exploit sim_trace_sim_th; try exact REL0; eauto. intro L1.
+            inv WRITE. inv WRITE1.
+            unfold Execution.label in EID0. ss.
+            rewrite PRE.(Valid.LABELS) in EID0.
+            rewrite IdMap.map_spec in EID0.
+            destruct (IdMap.find tid2 (Valid.aeus PRE)) eqn:FIND2; ss.
+            generalize (ATR tid2). intro ATR2. inv ATR2; try congr. des. simplify.
+            generalize (SIM tid2). intro SIM2. inv SIM2; simplify.
+            exploit sim_trace_last; try exact REL1. i. des. simplify.
+            exploit sim_trace_sim_th; try exact REL1; eauto. intro L2.
+            move H2 at bottom.
+            unfold v_gen in H2. ss.
+            rewrite <- H10, <- H16 in H2.
+            exploit L1.(WPROP2); eauto. i. des.
+            exploit L2.(WPROP2'); eauto. i. des.
+            exploit L1.(WPROP3); eauto. i. des.
+            exploit L2.(WPROP3); eauto. i. des.
+            rewrite x8, x15 in H2. inv H2.
+            rewrite H in x19. rewrite x12 in x19. inv x19. ss. }
+          subst.
+          inv WRITE. inv PO. ss. subst. inv H. inv H3. ss.
+        + rewrite H1. refl.
       - (* dob *)
         rename H1 into H.
         unfold Execution.dob in H. rewrite ? seq_assoc in *. des_union.
@@ -300,7 +405,42 @@ Proof.
           unfold v_gen. ss. rewrite <- H7. auto.
         }
         subst.
-        repeat rewrite <- join_r. ss.
+        repeat rewrite <- join_r. ss. unfold FwdItem.read_view. condtac; ss. clear X0. inv e.
+        generalize (L.(LC).(FWDBANK) (ValA.val vloc)). s. i. des.
+        + rewrite <- TS in H2.
+          destruct eid as [tid2 eid2], eid1 as [tid1 eid1].
+          assert (tid1 = tid2).
+          { inv H. exploit RF2; eauto. i. des.
+            inv WRITE0. rename EID0 into WRITE0.
+            unfold Execution.label in WRITE0. ss.
+            rewrite PRE.(Valid.LABELS) in WRITE0.
+            rewrite IdMap.map_spec in WRITE0.
+            destruct (IdMap.find tid1 (Valid.aeus PRE)) eqn:FIND1; ss.
+            generalize (ATR tid1). intro ATR1. inv ATR1; try congr. des. simplify.
+            generalize (SIM tid1). intro SIM1. inv SIM1; simplify.
+            exploit sim_trace_last; try exact REL0. i. des. simplify.
+            exploit sim_trace_sim_th; try exact REL0; eauto. intro L1.
+            inv WRITE. inv WRITE1.
+            unfold Execution.label in EID0. ss.
+            rewrite PRE.(Valid.LABELS) in EID0.
+            rewrite IdMap.map_spec in EID0.
+            destruct (IdMap.find tid2 (Valid.aeus PRE)) eqn:FIND2; ss.
+            generalize (ATR tid2). intro ATR2. inv ATR2; try congr. des. simplify.
+            generalize (SIM tid2). intro SIM2. inv SIM2; simplify.
+            exploit sim_trace_last; try exact REL1. i. des. simplify.
+            exploit sim_trace_sim_th; try exact REL1; eauto. intro L2.
+            move H2 at bottom.
+            unfold v_gen in H2. ss.
+            rewrite <- H10, <- H16 in H2.
+            exploit L1.(WPROP2); eauto. i. des.
+            exploit L2.(WPROP2'); eauto. i. des.
+            exploit L1.(WPROP3); eauto. i. des.
+            exploit L2.(WPROP3); eauto. i. des.
+            rewrite x8, x15 in H2. inv H2.
+            rewrite H in x19. rewrite x12 in x19. inv x19. ss. }
+          subst.
+          inv WRITE. inv PO. ss. subst. inv H. inv H3. ss.
+        + rewrite H1. refl.
       - (* dob *)
         rename H1 into H.
         unfold Execution.dob in H. rewrite ? seq_assoc in *. des_union.
