src/axiomatic/TsoPFtoA4SL.v
@@ -420,6 +420,24 @@ Proof.
         exploit EX2.(LABELS); eauto; ss.
         { rewrite List.app_length. s. lia. }
         rewrite List.nth_error_app2, Nat.sub_diag; ss. i. inv x0. inv LABEL.
+    + i. specialize (FWDBANK loc). des.
+      * left. esplits; eauto.
+        rewrite sim_local_fwd_step. econs.
+        econs; cycle 1.
+        { instantiate (1 := (_, _)). econs; ss. }
+        left. econs. split; eauto. econs; ss.
+        exploit EX2.(LABELS_REV); ss.
+        { apply nth_error_last. apply Nat.eqb_eq. ss. }
+        i. econs; eauto.
+      * right. esplits; eauto.
+        i. specialize (FWDBANK0 eid).
+        rewrite sim_local_fwd_none_step. rewrite inverse_step.
+        ii. inv H. inv REL.
+        { apply FWDBANK0. econs; eauto. }
+        { inv H. inv H1. exploit EX2.(LABELS); eauto; ss.
+          { rewrite List.app_length. s. lia. }
+          rewrite List.nth_error_app2, Nat.sub_diag; ss.
+          destruct l; ss. }
     + i. exploit PROMISES; eauto. i. des. esplits; cycle 1; eauto.
       inv N.
       * inv WRITE. exploit EX2.(LABELS); eauto; ss.
@@ -588,6 +606,43 @@ Proof.
         rewrite fun_add_spec.
         destruct (equiv_dec (ValA.val (sem_expr rmap1 eloc)) (ValA.val (sem_expr rmap1 eloc))) eqn:Heq1; ss.
         exfalso. apply c. ss.
+    + i. rewrite fun_add_spec. condtac; s.
+      { inversion e. subst. left. esplits; eauto.
+        - destruct ts; ss. clear. lia.
+        - instantiate (1 := (tid, length (ALocal.labels alc1))). econs.
+          + econs; ss.
+          + exploit EX2.(LABELS_REV); ss.
+            { apply nth_error_last. apply Nat.eqb_eq. ss. }
+            i. econs; eauto. inv VLOC. rewrite VAL0. apply Label.write_is_writing.
+          + i. inv PO. inv PO0. ss. subst. clear -N N0. lia.
+        - rewrite EX2.(XVEXT); cycle 1.
+          { ss. rewrite List.app_length. ss. clear. lia. }
+          destruct (length (ALocal.labels alc1) =? ALocal.next_eid alc1) eqn:Heq; cycle 1.
+          { rewrite Nat.eqb_neq in Heq. unfold ALocal.next_eid in Heq. ss. }
+          rewrite fun_add_spec.
+          destruct (equiv_dec (ValA.val (sem_expr rmap1 eloc)) (ValA.val (sem_expr rmap1 eloc))) eqn:Heq1; ss.
+      }
+      specialize (FWDBANK loc). des.
+      * left. esplits; eauto.
+        rewrite sim_local_fwd_step. econs.
+        econs; cycle 1.
+        { instantiate (1 := (_, _)). econs; ss. }
+        left. econs. split; eauto. econs; ss.
+        exploit EX2.(LABELS_REV); ss.
+        { apply nth_error_last. apply Nat.eqb_eq. ss. }
+        i. econs; eauto. ii. inv H.
+        destruct (equiv_dec (ValA.val (sem_expr armap1 eloc)) loc); ss. inv e.
+        inv VLOC. congr.
+      * right. esplits; eauto.
+        i. specialize (FWDBANK0 eid).
+        rewrite sim_local_fwd_none_step. rewrite inverse_step.
+        ii. inv H. inv REL.
+        { apply FWDBANK0. econs; eauto. }
+        { inv H. inv H1. exploit EX2.(LABELS); eauto; ss.
+          { rewrite List.app_length. s. lia. }
+            rewrite List.nth_error_app2, Nat.sub_diag; ss. i. inv x0. inv LABEL.
+            destruct (equiv_dec (ValA.val (sem_expr armap1 eloc)) loc); ss. inv e.
+            inv VLOC. congr. }
     + intro. rewrite Promises.unset_o. condtac; ss. i.
       exploit PROMISES; eauto. i. des. esplits; cycle 1; eauto.
       inv N.
@@ -789,6 +844,43 @@ Proof.
         { rewrite Nat.eqb_neq in Heq. unfold ALocal.next_eid in Heq. ss. }
         rewrite fun_add_spec. condtac; ss.
         exfalso. apply c. ss.
+    + i. rewrite fun_add_spec. condtac; s.
+      { inversion e. subst. left. esplits; eauto.
+        - destruct ts; ss. clear. lia.
+        - instantiate (1 := (tid, length (ALocal.labels alc1))). econs.
+          + econs; ss.
+          + exploit EX2.(LABELS_REV); ss.
+            { apply nth_error_last. apply Nat.eqb_eq. ss. }
+            i. econs; eauto. inv VLOC. rewrite VAL. apply Label.update_is_writing.
+          + i. inv PO. inv PO0. ss. subst. clear -N N0. lia.
+        - rewrite EX2.(XVEXT); cycle 1.
+          { ss. rewrite List.app_length. ss. clear. lia. }
+          destruct (length (ALocal.labels alc1) =? ALocal.next_eid alc1) eqn:Heq; cycle 1.
+          { rewrite Nat.eqb_neq in Heq. unfold ALocal.next_eid in Heq. ss. }
+          rewrite fun_add_spec.
+          destruct (equiv_dec (ValA.val (sem_expr rmap2 eloc)) (ValA.val (sem_expr rmap2 eloc))) eqn:Heq1; ss.
+      }
+      specialize (FWDBANK loc). des.
+      * left. esplits; eauto.
+        rewrite sim_local_fwd_step. econs.
+        econs; cycle 1.
+        { instantiate (1 := (_, _)). econs; ss. }
+        left. econs. split; eauto. econs; ss.
+        exploit EX2.(LABELS_REV); ss.
+        { apply nth_error_last. apply Nat.eqb_eq. ss. }
+        i. econs; eauto. ii. inv H.
+        destruct (equiv_dec (ValA.val (sem_expr armap2 eloc)) loc); ss. inv e.
+        inv VLOC. congr.
+      * right. esplits; eauto.
+        i. specialize (FWDBANK0 eid).
+        rewrite sim_local_fwd_none_step. rewrite inverse_step.
+        ii. inv H. inv REL.
+        { apply FWDBANK0. econs; eauto. }
+        { inv H. inv H1. exploit EX2.(LABELS); eauto; ss.
+          { rewrite List.app_length. s. lia. }
+            rewrite List.nth_error_app2, Nat.sub_diag; ss. i. inv x0. inv LABEL.
+            destruct (equiv_dec (ValA.val (sem_expr armap2 eloc)) loc); ss. inv e.
+            inv VLOC. congr. }
     + intro. rewrite Promises.unset_o. condtac; ss. i.
       exploit PROMISES; eauto. i. des. esplits; cycle 1; eauto.
       inv N.
@@ -1129,6 +1221,24 @@ Proof.
         exploit EX2.(LABELS); eauto; ss.
         { rewrite List.app_length. s. lia. }
         rewrite List.nth_error_app2, Nat.sub_diag; ss. i. inv x0. inv LABEL.
+    + i. specialize (FWDBANK loc). des.
+      * left. esplits; eauto.
+        rewrite sim_local_fwd_step. econs.
+        econs; cycle 1.
+        { instantiate (1 := (_, _)). econs; ss. }
+        left. econs. split; eauto. econs; ss.
+        exploit EX2.(LABELS_REV); ss.
+        { apply nth_error_last. apply Nat.eqb_eq. ss. }
+        i. econs; eauto.
+      * right. esplits; eauto.
+        i. specialize (FWDBANK0 eid).
+        rewrite sim_local_fwd_none_step. rewrite inverse_step.
+        ii. inv H. inv REL.
+        { apply FWDBANK0. econs; eauto. }
+        { inv H. inv H1. exploit EX2.(LABELS); eauto; ss.
+          { rewrite List.app_length. s. lia. }
+          rewrite List.nth_error_app2, Nat.sub_diag; ss.
+          destruct l; ss. }
     + i. exploit PROMISES; eauto. i. des. esplits; cycle 1; eauto.
       inv N.
       * inv WRITE. exploit EX2.(LABELS); eauto; ss.
@@ -1226,6 +1336,26 @@ Proof.
         exploit EX2.(LABELS); eauto; ss.
         { rewrite List.app_length. s. lia. }
         rewrite List.nth_error_app2, Nat.sub_diag; ss. i. inv x0. inv LABEL.
+    + i. specialize (FWDBANK loc). des.
+      * left. esplits; eauto.
+        rewrite List.app_length, Nat.add_1_r.
+        rewrite sim_local_fwd_step. econs.
+        econs; cycle 1.
+        { instantiate (1 := (_, _)). econs; ss. }
+        left. econs. split; eauto. econs; ss.
+        exploit EX2.(LABELS_REV); ss.
+        { apply nth_error_last. apply Nat.eqb_eq. ss. }
+        intro X. econs; eauto.
+      * right. esplits; eauto.
+        i. specialize (FWDBANK0 eid).
+        rewrite List.app_length, Nat.add_1_r.
+        rewrite sim_local_fwd_none_step. rewrite inverse_step.
+        ii. inv H. inv REL.
+        { apply FWDBANK0. econs; eauto. }
+        { inv H. inv H1. exploit EX2.(LABELS); eauto; ss.
+          { rewrite List.app_length. s. lia. }
+          rewrite List.nth_error_app2, Nat.sub_diag; ss.
+          destruct l; ss. }
     + i. exploit PROMISES; eauto. i. des. esplits; cycle 1; eauto.
       rewrite List.app_length, Nat.add_1_r. inv N.
       * inv WRITE. exploit EX2.(LABELS); eauto; ss.
